Improve the source level small-step semantics
- Use explicit continuations
- Prove correctness of the functional step w.r.t. the semantics
- Prove determinism of the semantics

Source/CS.v
@@ -5,218 +5,196 @@ Require Import Common.Values.
 Require Import Common.Memory.
 Require Import Source.Language.
 Require Import Source.GlobalEnv.
+Require Import Lib.Tactics.
 
-(* small-step semantics with evaluation contexts *)
+Inductive cont : Type :=
+| Kstop
+| Kbinop1 (op: binop) (re: expr) (k: cont)
+| Kbinop2 (op: binop) (lv: value) (k: cont)
+| Kseq (e: expr) (k: cont)
+| Kif (e1: expr) (e2: expr) (k: cont)
+| Kalloc (k: cont)
+| Kderef (k: cont)
+| Kassign1 (e: expr) (k: cont)
+| Kassign2 (v: value) (k: cont)
+| Kcall (C: Component.id) (P: Procedure.id) (k: cont).
 
-Inductive eval_context : Type :=
-| EC_binop_left : binop -> expr -> eval_context
-| EC_binop_right : binop -> value -> eval_context
-| EC_seq_right : expr -> eval_context
-| EC_if : expr -> expr -> eval_context
-| EC_alloc : eval_context
-| EC_deref : eval_context
-| EC_assign_right : expr -> eval_context
-| EC_assign_left : value -> eval_context
-| EC_call : Component.id -> Procedure.id -> eval_context.
+Definition stack : Type := list (Component.id * value * cont).
+Definition state : Type := Component.id * stack * Memory.t * cont * expr.
 
-Definition kont : Type := list eval_context.
-Definition stack : Type := list (Component.id * value * kont).
-Definition state : Type := Component.id * stack * Memory.t * kont * expr.
+Inductive kstep (G: global_env) : state -> trace -> state -> Prop :=
+| KS_Binop1 : forall C s mem k op e1 e2,
+    let t := E0 in
+    kstep G (C, s, mem, k, E_binop op e1 e2)
+          t (C, s, mem, Kbinop1 op e2 k, e1)
+| KS_Binop2 : forall C s mem k op v1 e2,
+    let t := E0 in
+    kstep G (C, s, mem, Kbinop1 op e2 k, E_val v1)
+          t (C, s, mem, Kbinop2 op v1 k, e2)
+| KS_BinopEval : forall C s mem k op v1 v2,
+    let t := E0 in
+    kstep G (C, s, mem, Kbinop2 op v1 k, E_val v2)
+          t (C, s, mem, k, E_val (eval_binop op v1 v2))
+| KS_Seq1 :  forall C s mem k e1 e2,
+    let t := E0 in
+    kstep G (C, s, mem, k, E_seq e1 e2)
+          t (C, s, mem, Kseq e2 k, e1)
+| KS_Seq2 : forall C s mem k v e2,
+    let t := E0 in
+    kstep G (C, s, mem, Kseq e2 k, E_val v)
+          t (C, s, mem, k, e2)
+| KS_If : forall C s mem k e1 e2 e3,
+    let t := E0 in
+    kstep G (C, s, mem, k, E_if e1 e2 e3)
+          t (C, s, mem, Kif e2 e3 k, e1)
+| KS_IfTrue : forall C s mem k e2 e3 i,
+    i <> 0 ->
+    let t := E0 in
+    kstep G (C, s, mem, Kif e2 e3 k, E_val (Int i))
+          t (C, s, mem, k, e2)
+| KS_IfFalse : forall C s mem k e2 e3,
+    let t := E0 in
+    kstep G (C, s, mem, Kif e2 e3 k, E_val (Int 0))
+          t (C, s, mem, k, e3)
+| KS_LocalBuffer : forall C s mem k b,
+    NMap.find C (genv_buffers G) = Some b ->
+    let t := E0 in
+    kstep G (C, s, mem, k, E_local)
+          t (C, s, mem, k, E_val (Ptr (C,b,0)))
+| KS_Alloc1 : forall C s mem k e,
+    let t := E0 in
+    kstep G (C, s, mem, k, E_alloc e)
+          t (C, s, mem, Kalloc k, e)
+| KS_AllocEval : forall C s mem mem' k size ptr,
+    Memory.alloc mem C size = Some (mem', ptr) ->
+    let t := E0 in
+    kstep G (C, s, mem, Kalloc k, E_val (Int size))
+          t (C, s, mem', k, E_val (Ptr ptr))
+| KS_Deref1 : forall C s mem k e,
+    let t := E0 in
+    kstep G (C, s, mem, k, E_deref e)
+          t (C, s, mem, Kderef k, e)
+| KS_DerefEval : forall C s mem k C' b' o' v,
+    Memory.load mem (C',b',o') = Some v ->
+    let t := E0 in
+    kstep G (C, s, mem, Kderef k, E_val (Ptr (C',b',o')))
+          t (C, s, mem, k, E_val v)
+| KS_Assign1 : forall C s mem k e1 e2,
+    let t := E0 in
+    kstep G (C, s, mem, k, E_assign e1 e2)
+          t (C, s, mem, Kassign1 e1 k, e2)
+| KS_Assign2 : forall C s mem k v e1,
+    let t := E0 in
+    kstep G (C, s, mem, Kassign1 e1 k, E_val v)
+          t (C, s, mem, Kassign2 v k, e1)
+| KS_AssignEval : forall C s mem mem' k v C' b' o',
+    C = C' ->
+    Memory.store mem (C',b',o') v = Some mem' ->
+    let t := E0 in
+    kstep G (C, s, mem, Kassign2 v k, E_val (Ptr (C',b',o')))
+          t (C, s, mem', k, E_val v)
+| KS_Call1 : forall C s mem k C' P e,
+    imported_procedure (genv_interface G) C C' P \/ C = C' ->
+    let t := E0 in
+    kstep G (C, s, mem, k, E_call C' P e)
+          t (C, s, mem, Kcall C' P k, e)
+| KS_Call2 : forall C s mem mem' k C' P v C'_procs P_expr b b' old_call_arg,
+    (* retrieve the procedure code *)
+    NMap.find C' (genv_procedures G) = Some C'_procs ->
+    NMap.find P C'_procs = Some P_expr ->
+    (* save the old call argument *)
+    NMap.find C (genv_buffers G) = Some b ->
+    Memory.load mem (C,b,0) = Some old_call_arg ->
+    (* place the call argument in the target memory *)
+    NMap.find C' (genv_buffers G) = Some b' ->
+    Memory.store mem (C',b',0) (Int v) = Some mem' ->
+    let t := [ECall C P v C'] in
+    kstep G (C, s, mem, Kcall C' P k, E_val (Int v))
+          t (C', (C, old_call_arg, k) :: s, mem', Kstop, P_expr)
+| KS_CallRet : forall C s mem mem' k v C' old_call_arg b,
+    (* restore the old call argument *)
+    NMap.find C' (genv_buffers G) = Some b ->
+    Memory.store mem (C', b, 0) old_call_arg = Some mem' ->
+    let t := [ERet C v C'] in
+    kstep G (C, (C', old_call_arg, k) :: s, mem, Kstop, E_val (Int v))
+          t (C', s, mem', k, E_val (Int v)).
 
-Inductive step (G : global_env) : state -> trace -> state -> Prop :=
-| S_binop_push_left:
-    forall C s mem ks b_op e1 e2,
-      let st := (C, s, mem, ks, E_binop b_op e1 e2) in
-      let st' := (C, s, mem, EC_binop_left b_op e2 :: ks, e1) in
-      step G st E0 st'
-| S_binop_push_right:
-    forall C s mem ks b_op v1 e2,
-      let st := (C, s, mem, EC_binop_left b_op e2 :: ks, E_val v1) in
-      let st' := (C, s, mem, EC_binop_right b_op v1 :: ks, e2) in
-      step G st E0 st'
-| S_binop_pop:
-    forall C s mem ks b_op v1 v2,
-      let st := (C, s, mem, EC_binop_right b_op v1 :: ks, E_val v2) in
-      let st' := (C, s, mem, ks, E_val (eval_binop b_op v1 v2)) in
-      step G st E0 st'
-| S_seq_push:
-    forall C s mem ks e1 e2,
-      let st := (C, s, mem, ks, E_seq e1 e2) in
-      let st' := (C, s, mem, EC_seq_right e2 :: ks, e1) in
-      step G st E0 st'
-| S_seq_pop:
-    forall C s mem ks v e2,
-      let st := (C, s, mem, EC_seq_right e2 :: ks, E_val v) in
-      let st' := (C, s, mem, ks, e2) in
-      step G st E0 st'
-| S_if_push:
-    forall C s mem ks e1 e2 e3,
-      let st := (C, s, mem, ks, E_if e1 e2 e3) in
-      let st' := (C, s, mem, EC_if e2 e3 :: ks, e1) in
-      step G st E0 st'
-| S_if_pop_conseq:
-    forall C s mem ks e2 e3 i,
-      let st := (C, s, mem, EC_if e2 e3 :: ks, E_val (Int i)) in
-      i <> 0 ->
-      let st' := (C, s, mem, ks, e2) in
-      step G st E0 st'
-| S_if_pop_alt:
-    forall C s mem ks e2 e3,
-      let st := (C, s, mem, EC_if e2 e3 :: ks, E_val (Int 0)) in
-      let st' := (C, s, mem, ks, e3) in
-      step G st E0 st'
-| S_local_buffer:
-    forall C s mem ks b,
-      let st := (C, s, mem, ks, E_local) in
-      NMap.find C (genv_buffers G) = Some b ->
-      let st' := (C, s, mem, ks, E_val (Ptr (C,b,0))) in
-      step G st E0 st'
-| S_alloc_push:
-    forall C s mem ks e,
-      let st := (C, s, mem, ks, E_alloc e) in
-      let st' := (C, s, mem, EC_alloc :: ks, e) in
-      step G st E0 st'
-| S_alloc_pop:
-    forall C s mem mem' ks size ptr,
-      let st := (C, s, mem, EC_alloc :: ks, E_val (Int size)) in
-      Memory.alloc mem C size = Some (mem', ptr) ->
-      let st' := (C, s, mem', ks, E_val (Ptr ptr)) in
-      step G st E0 st'
-| S_deref_push:
-    forall C s mem ks e,
-      let st := (C, s, mem, ks, E_deref e) in
-      let st' := (C, s, mem, EC_deref :: ks, e) in
-      step G st E0 st'
-| S_deref_pop:
-    forall C s mem ks C' b' o' v,
-      let st := (C, s, mem, EC_deref :: ks, E_val (Ptr (C',b',o'))) in
-      Memory.load mem (C',b',o') = Some v ->
-      let st' := (C, s, mem, ks, E_val v) in
-      step G st E0 st'
-| S_assign_push_arg:
-    forall C s mem ks e1 e2,
-      let st := (C, s, mem, ks, E_assign e1 e2) in
-      let st' := (C, s, mem, EC_assign_right e2 :: ks, e1) in
-      step G st E0 st'
-| S_assign_push_dest:
-    forall C s mem ks v e2,
-      let st := (C, s, mem, EC_assign_right e2 :: ks, E_val v) in
-      let st' := (C, s, mem, EC_assign_left v :: ks, e2) in
-      step G st E0 st'
-| S_assign_pop:
-    forall C s mem mem' ks v C' b' o',
-      let st := (C, s, mem, EC_assign_left v :: ks, E_val (Ptr (C',b',o'))) in
-      C = C' ->
-      Memory.store mem (C',b',o') v = Some mem' ->
-      let st' := (C, s, mem', ks, E_val v) in
-      step G st E0 st'
-| S_call_push_arg:
-    forall C s mem ks C' P e,
-      let st := (C, s, mem, ks, E_call C' P e) in
-      imported_procedure (genv_interface G) C C' P \/ C = C' ->
-      let st' := (C, s, mem, EC_call C' P :: ks, e) in
-      step G st E0 st'
-| S_call_push_proc:
-    forall C s mem mem' ks C' P v C'_procs P_expr b b' old_call_arg,
-      let st := (C, s, mem, EC_call C' P :: ks, E_val (Int v)) in
-      (* retrieve the procedure code *)
-      NMap.find C' (genv_procedures G) = Some C'_procs ->
-      NMap.find P C'_procs = Some P_expr ->
-      (* save the old call argument *)
-      NMap.find C (genv_buffers G) = Some b ->
-      Memory.load mem (C,b,0) = Some old_call_arg ->
-      (* place the call argument in the target memory *)
-      NMap.find C' (genv_buffers G) = Some b' ->
-      Memory.store mem (C',b',0) (Int v) = Some mem' ->
-      let st' := (C', (C, old_call_arg, ks) :: s, mem', [], P_expr) in
-      let t := [ECall C P v C'] in
-      step G st t st'
-| S_call_pop:
-    forall C s mem mem' ks v C' old_call_arg b,
-      let st := (C, (C',old_call_arg,ks) :: s, mem, [], E_val (Int v)) in
-      (* restore the old call argument *)
-      NMap.find C' (genv_buffers G) = Some b ->
-      Memory.store mem (C',b,0) old_call_arg = Some mem' ->
-      let st' := (C', s, mem', ks, E_val (Int v)) in
-      let t := [ERet C v C'] in
-      step G st t st'.
+(* functional kstep *)
 
-(* functional version of step *)
-
-Definition eval_step (G : global_env) (st : state) : option (trace * state) :=
-  let '(C, s, mem, ks, e) := st in
+Definition eval_kstep (G : global_env) (st : state) : option (trace * state) :=
+  let '(C, s, mem, k, e) := st in
   match e with
   (* pushing a new continuation *)
   | E_binop b_op e1 e2 =>
-    Some (E0, (C, s, mem, EC_binop_left b_op e2 :: ks, e1))
+    Some (E0, (C, s, mem, Kbinop1 b_op e2 k, e1))
   | E_seq e1 e2 =>
-    Some (E0, (C, s, mem, EC_seq_right e2 :: ks, e1))
+    Some (E0, (C, s, mem, Kseq e2 k, e1))
   | E_if e1 e2 e3 =>
-    Some (E0, (C, s, mem, EC_if e2 e3 :: ks, e1))
+    Some (E0, (C, s, mem, Kif e2 e3 k, e1))
   | E_local =>
     match NMap.find C (genv_buffers G) with
-    | Some b => Some (E0, (C, s, mem, ks, E_val (Ptr (C,b,0))))
+    | Some b => Some (E0, (C, s, mem, k, E_val (Ptr (C,b,0))))
     | None => None
     end
   | E_alloc e =>
-    Some (E0, (C, s, mem, EC_alloc :: ks, e))
+    Some (E0, (C, s, mem, Kalloc k, e))
   | E_deref e =>
-    Some (E0, (C, s, mem, EC_deref :: ks, e))
+    Some (E0, (C, s, mem, Kderef k, e))
   | E_assign e1 e2 =>
-    Some (E0, (C, s, mem, EC_assign_right e2 :: ks, e1))
+    Some (E0, (C, s, mem, Kassign1 e1 k, e2))
   | E_call C' P e =>
     if (imported_procedure_b (genv_interface G) C C' P) || (C =? C') then
-      Some (E0, (C, s, mem, EC_call C' P :: ks, e))
+      Some (E0, (C, s, mem, Kcall C' P k, e))
     else
       None
   (* evaluating current continuation *)
   | E_val v =>
-    match ks with
-    | EC_binop_left b_op e2 :: ks' =>
-      Some (E0, (C, s, mem, EC_binop_right b_op v :: ks', e2))
-    | EC_binop_right b_op v1 :: ks' =>
-      Some (E0, (C, s, mem, ks', E_val (eval_binop b_op v1 v)))
-    | EC_seq_right e2 :: ks' =>
-      Some (E0, (C, s, mem, ks', e2))
-    | EC_if e2 e3 :: ks' =>
+    match k with
+    | Kbinop1 b_op e2 k' =>
+      Some (E0, (C, s, mem, Kbinop2 b_op v k', e2))
+    | Kbinop2 b_op v1 k' =>
+      Some (E0, (C, s, mem, k', E_val (eval_binop b_op v1 v)))
+    | Kseq e2 k' =>
+      Some (E0, (C, s, mem, k', e2))
+    | Kif e2 e3 k' =>
       match v with
-      | Int 0 => Some (E0, (C, s, mem, ks', e3))
-      | Int i => Some (E0, (C, s, mem, ks', e2))
+      | Int 0 => Some (E0, (C, s, mem, k', e3))
+      | Int i => Some (E0, (C, s, mem, k', e2))
       | _ => None
       end
-    | EC_alloc :: ks' =>
+    | Kalloc k' =>
       match v with
       | Int size =>
         match Memory.alloc mem C size with
-        | Some (mem',ptr) => Some (E0, (C, s, mem', ks', E_val (Ptr ptr)))
+        | Some (mem',ptr) => Some (E0, (C, s, mem', k', E_val (Ptr ptr)))
         | None => None
         end
       | _ => None
       end
-    | EC_deref :: ks' =>
+    | Kderef k' =>
       match v with
       | Ptr (C',b',o') =>
         match Memory.load mem (C',b',o') with
-        | Some v => Some (E0, (C, s, mem, ks', E_val v))
+        | Some v => Some (E0, (C, s, mem, k', E_val v))
         | None => None
         end
       | _ => None
       end
-    | EC_assign_right e2 :: ks' =>
-      Some (E0, (C, s, mem, EC_assign_left v :: ks', e2))
-    | EC_assign_left v' :: ks' =>
+    | Kassign1 e1 k' =>
+      Some (E0, (C, s, mem, Kassign2 v k', e1))
+    | Kassign2 v' k' =>
       match v with
       | Ptr (C',b',o') =>
         if C =? C' then
           match Memory.store mem (C',b',o') v' with
-          | Some mem' => Some (E0, (C, s, mem', ks', E_val v'))
+          | Some mem' => Some (E0, (C, s, mem', k', E_val v'))
           | None => None
           end
         else
           None
       | _ => None
       end
-    | EC_call C' P :: ks' =>
+    | Kcall C' P k' =>
       match v with
       | Int i =>
         (* retrieve the procedure code *)
@@ -235,7 +213,7 @@ Definition eval_step (G : global_env) (st : state) : option (trace * state) :=
                   match Memory.store mem (C',b',0) (Int i) with
                   | Some mem' =>
                     let t := [ECall C P i C'] in
-                    Some (t, (C', (C, old_call_arg, ks') :: s, mem', [], P_expr))
+                    Some (t, (C', (C, old_call_arg, k') :: s, mem', Kstop, P_expr))
                   | None => None
                   end
                 | None => None
@@ -250,16 +228,16 @@ Definition eval_step (G : global_env) (st : state) : option (trace * state) :=
         end
       | _ => None
       end
-    | [] =>
+    | Kstop =>
       match v, s with
-      | Int i, (C',old_call_arg,ks) :: s' =>
+      | Int i, (C',old_call_arg,k') :: s' =>
         (* restore the old call argument *)
         match NMap.find C' (genv_buffers G) with
         | Some b =>
           match Memory.store mem (C',b,0) old_call_arg with
           | Some mem' =>
             let t := [ERet C i C'] in
-            Some (t, (C', s', mem', ks, E_val (Int i)))
+            Some (t, (C', s', mem', k', E_val (Int i)))
           | None => None
           end
         | None => None
@@ -270,12 +248,28 @@ Definition eval_step (G : global_env) (st : state) : option (trace * state) :=
   | _ => None
   end.
 
-Theorem step_implies_eval_step:
+Ltac rewrite_equalities :=
+  match goal with 
+  | H: (_ =? _) = true |- _ => apply beq_nat_true_iff in H; rewrite H
+  end.
+
+Ltac unfold_state :=
+  match goal with
+  | H: state |- _ =>
+    let C := fresh "C" in
+    let s := fresh "s" in
+    let mem := fresh "mem" in
+    let k := fresh "k" in
+    let e := fresh "e" in
+    destruct H as [[[[C s] mem] k] e]
+  end.
+
+Theorem eval_kstep_complete:
   forall G st t st',
-    step G st t st' -> eval_step G st =  Some (t, st').
+    kstep G st t st' -> eval_kstep G st =  Some (t, st').
 Proof.
-  intros G st t st' Hstep.
-  inversion Hstep; subst; simpl; auto.
+  intros G st t st' Hkstep.
+  inversion Hkstep; subst; simpl; auto.
   (* if expressions *)
   - apply beq_nat_false_iff in H.
     destruct i eqn:Hi; auto.
@@ -285,16 +279,14 @@ Proof.
   (* memory allocs *)
   - rewrite H. auto.
   (* memory loads *)
-  - unfold Memory.load in H.
-    destruct (NMap.find (elt:=ComponentMemory.t) C' mem) eqn:HC'mem.
-    + rewrite H. auto.
-    + inversion H.
+  - unfold Memory.store, Memory.load, Memory.alloc in *.
+    repeat simplify_options.
+    reflexivity.
   (* memory stores *)
-  - rewrite <- beq_nat_refl.
-    unfold Memory.store in H0.
-    destruct (NMap.find (elt:=ComponentMemory.t) C' mem) eqn:HC'mem.
-    + rewrite H0. auto.
-    + inversion H0.
+  - unfold Memory.store, Memory.load, Memory.alloc in *.
+    rewrite <- beq_nat_refl.
+    repeat simplify_options.
+    reflexivity.
   (* calls/returns *)
   - destruct H.
     + destruct H as [CI [HCI Himport]].
@@ -306,32 +298,71 @@ Proof.
       inversion Himport.
       * rewrite <- H0. simpl. auto.
       * rewrite <- H. simpl. auto.
-    + unfold st'0. rewrite H. rewrite <- beq_nat_refl.
+    + rewrite H. rewrite <- beq_nat_refl.
       rewrite orb_true_r. auto.
-  - rewrite H, H0, H1, H3.
-    unfold Memory.load in H2.
-    destruct (NMap.find (elt:=ComponentMemory.t) C mem) eqn:HCmem.
-    + rewrite H2.
-      unfold Memory.store in H4.
-      destruct (NMap.find (elt:=ComponentMemory.t) C' mem) eqn:HC'mem.
-      * inversion HCmem. subst. rewrite H4. auto.
-      * inversion H4.
-    + inversion H2.
-  - rewrite H.
-    unfold Memory.store in H0.
-    destruct (NMap.find (elt:=ComponentMemory.t) C' mem) eqn:HC'mem.
-    + rewrite H0. auto.
-    + inversion H0.
+  - unfold Memory.store, Memory.load, Memory.alloc in *.
+    repeat simplify_options.
+    reflexivity.
+  - unfold Memory.store, Memory.load, Memory.alloc in *.
+    repeat simplify_options.
+    reflexivity.
 Qed.
 
-Theorem step_determinism:
-  forall G st t st1 st2,
-    step G st t st1 -> step G st t st2 -> st1 = st2.
+Theorem eval_kstep_sound:
+  forall G st t st',
+    eval_kstep G st =  Some (t, st') -> kstep G st t st'.
 Proof.
-  intros G st t st1 st2 Hstep1 Hstep2.
-  apply step_implies_eval_step in Hstep1.
-  apply step_implies_eval_step in Hstep2.
-  rewrite Hstep1 in Hstep2.
-  inversion Hstep2.
-  auto.
+  intros.
+  repeat unfold_state.
+  match goal with
+  | H: eval_kstep _ _ = Some _ |- kstep _ (_, _, _, _, ?E) _ (_, _, _, _, _) =>
+    destruct E; simpl in H;
+      try discriminate;
+      try (repeat simplify_options;
+           econstructor; eauto;
+           repeat rewrite_memory_operations;
+           repeat rewrite_equalities;
+           reflexivity)
+  end.
+  - repeat simplify_options.
+    rewrite orb_true_iff in Heqb.
+    rewrite beq_nat_true_iff in Heqb.
+    econstructor.
+    destruct Heqb.
+    + left.
+      unfold imported_procedure.
+      unfold Program.has_component, Component.is_importing.
+      unfold imported_procedure_b in *.
+      destruct (NMap.find (elt:=Component.interface) C (genv_interface G)) eqn:Hi;
+        inversion H; try discriminate.
+      exists i1. split.
+      * apply (NMap.find_2 Hi).
+      * destruct (count_occ procs_eqdec (Component.import i1) (i, i0) =? 0) eqn:Hcount;
+           inversion H; try discriminate.
+         apply count_occ_In with procs_eqdec.
+         rewrite beq_nat_false_iff in Hcount.
+         apply Nat.neq_0_lt_0 in Hcount.
+         unfold gt. auto.
+    + right. auto.
+Qed.
+
+Theorem eval_kstep_correct:
+  forall G st t st',
+    eval_kstep G st =  Some (t, st') <-> kstep G st t st'.
+Proof.
+  split.
+  apply eval_kstep_sound.
+  apply eval_kstep_complete.
+Qed.
+
+Theorem kstep_deterministic:
+  forall G st t st1 st2,
+    kstep G st t st1 -> kstep G st t st2 -> st1 = st2.
+Proof.
+  intros G st t st1 st2 Hkstep1 Hkstep2.
+  apply eval_kstep_correct in Hkstep1.
+  apply eval_kstep_correct in Hkstep2.
+  rewrite Hkstep1 in Hkstep2.
+  inversion Hkstep2.
+  reflexivity.
 Qed.
