Lib/Tactics.v
@@ -1,0 +1,22 @@
+Require Import Common.Maps.
+Require Import Common.Memory.
+
+Ltac inv H :=
+  inversion H; clear H; subst.
+
+Ltac simplify_options :=
+  match goal with
+  | H: Some ?x1 = Some ?x2 |- _ => inv H
+  | |- match ?V with _ => _ end = Some _ =>
+    destruct V eqn:?; subst; try discriminate
+  | H: match ?V with _ => _ end = Some _ |- _ =>
+    destruct V eqn:?; inv H
+  end.
+
+Ltac rewrite_memory_operations :=
+  unfold Memory.alloc, Memory.load, Memory.store;
+  match goal with
+  | H: NMap.find (elt:=ComponentMemory.t) _ _ = Some _ |- _ => rewrite H
+  | H: ComponentMemory.store _ _ _ _ = Some _ |- _ => rewrite H
+  | H: ComponentMemory.load _ _ _ = Some _ |- _ => rewrite H
+  end.
